theories/models/utp_cml/utp_cml_tac.thy
@@ -13,14 +13,78 @@ imports
   utp_cml_functions
 begin
 
+text {* Theorem Attributes *}
+
+ML {*
+  structure cmlty_defs =
+    Named_Thms (val name = @{binding cmlty_defs} val description = "CML type defs")
+*}
+
+ML {*
+  structure cmlval_defs =
+    Named_Thms (val name = @{binding cmlval_defs} val description = "CML value defs")
+*}
+
+ML {*
+  structure cmlfun_defs =
+    Named_Thms (val name = @{binding cmlfun_defs} val description = "CML function defs")
+*}
+
+ML {*
+  structure cmlchan_defs =
+    Named_Thms (val name = @{binding cmlchan_defs} val description = "CML channel defs")
+*}
+
+ML {*
+  structure cmlproc_defs =
+    Named_Thms (val name = @{binding cmlproc_defs} val description = "CML process defs")
+*}
+
+ML {*
+  structure cmlop_defs =
+    Named_Thms (val name = @{binding cmlop_defs} val description = "CML operation defs")
+*}
+
+ML {*
+  structure cmlact_defs =
+    Named_Thms (val name = @{binding cmlact_defs} val description = "CML action defs")
+*}
+
+setup cmlty_defs.setup
+setup cmlval_defs.setup
+setup cmlfun_defs.setup
+setup cmlchan_defs.setup
+setup cmlproc_defs.setup
+setup cmlop_defs.setup
+setup cmlact_defs.setup
+
+ML {*
+  fun utp_cml_defs ctxt =
+    (simpset_of ctxt)
+      addsimps (cmlty_defs.get ctxt)
+      addsimps (cmlval_defs.get ctxt)
+      addsimps (cmlfun_defs.get ctxt)
+      addsimps (cmlchan_defs.get ctxt)
+      addsimps (cmlproc_defs.get ctxt)
+      addsimps (cmlop_defs.get ctxt)
+      addsimps (cmlact_defs.get ctxt)
+      addsimps (uop_defs.get ctxt);
+*}
 
 ML {*
   fun utp_cml_simpset ctxt =
-    (simpset_of ctxt)
+    (utp_cml_defs ctxt)
       addsimps (evalp.get ctxt)
+      addsimps (evalpp.get ctxt)
       addsimps (closure.get ctxt)
       addsimps (typing.get ctxt)
       addsimps (defined.get ctxt);
+*}
+
+ML {*
+  fun utp_cml_unfold_tac thms ctxt i =
+    CHANGED (
+      TRY (asm_full_simp_tac (utp_cml_defs ctxt) i))
 *}
 
 ML {*
@@ -36,6 +100,12 @@ ML {*
       (asm_full_simp_tac (simpset_of ctxt)) THEN_ALL_NEW
       (SELECT_GOAL (auto_tac ctxt))) i)
 *}
+
+method_setup unfold_cml = {*
+  Attrib.thms >>
+  (fn thms => fn ctxt =>
+    SIMPLE_METHOD' (utp_cml_unfold_tac thms ctxt))
+*} "proof tactic for CML"
 
 method_setup cml_tac = {*
   Attrib.thms >>
